src/Rupicola/Examples/Echo/IO.v
@@ -1,111 +1,179 @@
 Require Import Rupicola.Lib.Api.
-Require Coq.Logic.Eqdep Coq.Logic.FunctionalExtensionality.
+Require Coq.Logic.Eqdep Coq.Logic.FunctionalExtensionality Coq.Sets.Ensembles.
 Open Scope list_scope.
 
-Inductive Free {F: Type -> Type} {A: Type} : Type :=
-| Pure (a: A) : Free
-| Impure {X} (f: F X) (k: X -> Free) : Free.
-Arguments Free: clear implicits.
+Set Implicit Arguments.
 
-Definition Call {F} {A} (f: F A) := Impure f Pure.
+Class Monad (M: Type -> Type) :=
+  { mret {A} : A -> M A;
+    mbind {A B} : M A -> (A -> M B) -> M B;
+    mbindn {A B} (vars: list string) (ma: M A) (kA: A -> M B) : M B :=
+      mbind ma kA;
 
-Module FreeMonad.
-  Section FreeMonad.
+    mbind_mret {A} (ma: M A) : mbind ma mret = ma;
+    mret_mbind {A B} a (k: A -> M B) : mbind (mret a) k = k a;
+    mbind_mbind {A B C} ma (ka: A -> M B) (kb: B -> M C) :
+      mbind (mbind ma ka) kb = mbind ma (fun a => mbind (ka a) kb) }.
+
+Module Free.
+  Section Free.
     Context {F: Type -> Type}.
-    Notation Free := (Free F).
 
-    Definition ret {A} (a: A) : Free A := Pure a.
-    Fixpoint bind {A B} (f: Free A) (kA: A -> Free B) : Free B :=
+    Inductive M (A: Type) : Type :=
+    | Pure (a: A) : M A
+    | Impure X (f: F X) (k: X -> M A) : M A.
+
+    Definition Call {A} (f: F A) := Impure f (@Pure _).
+
+    Definition ret {A} (a: A) : M A := Pure a.
+
+    Fixpoint bind {A B} (f: M A) (kA: A -> M B) : M B :=
       match f with
       | Pure a => kA a
       | Impure f kX => Impure f (fun x => bind (kX x) kA)
       end.
-    Definition bindn {A B} (vars: list string) (a: Free A) (kA: A -> Free B) : Free B :=
-      bind a kA.
 
     Ltac s :=
-      simpl; try reflexivity;
-      eauto using f_equal, FunctionalExtensionality.functional_extensionality.
+      simpl; eauto using f_equal, FunctionalExtensionality.functional_extensionality.
 
-    Definition bind_ret {A} (ca: Free A) :
-      bind ca ret = ca.
-    Proof. induction ca; s. Qed.
+    Global Program Instance MonadM : Monad M :=
+      {| mret := @ret;
+         mbind := @bind |}.
+    Obligation 1. Proof. induction ma; s. Qed.
+    Obligation 3. Proof. induction ma; s. Qed.
 
-    Definition ret_bind {A B} a (k: A -> Free B) :
-      bind (ret a) k = k a.
-    Proof. s. Qed.
+    Context {M': Type -> Type} {MM': Monad M'}.
+    Context (interpF: forall {A}, F A -> M' A).
 
-    Definition bind_bind {A B C}
-               ca (ka: A -> Free B) (kb: B -> Free C) :
-      bind (bind ca ka) kb =
-      bind ca (fun a => bind (ka a) kb).
-    Proof. induction ca; s. Qed.
-
-    Context (M: Type -> Type).
-    Context (retM: forall {A}, A -> M A).
-    Context (bindM: forall {A B}, (M A) -> (A -> M B) -> M B).
-    Context (interpF: forall A, F A -> M A).
-
-    Fixpoint interp {A: Type} (f: Free A) : M A :=
+    Fixpoint interp {A: Type} (f: M A) : M' A :=
       match f with
-      | Pure a => @retM _ a
-      | Impure f k => @bindM _ _ (@interpF _ f) (fun x => interp (k x))
+      | Pure a => mret a
+      | Impure f k => mbind (@interpF _ f) (fun x => interp (k x))
       end.
-  End FreeMonad.
-End FreeMonad.
 
-Module IOMonad.
-  Section IOMonad.
-  Export FreeMonad.
-  Context {T: Type}.
+    Lemma interp_bind {A B}:
+      forall (ma: M A) (k: A -> M B),
+        mbind (M := M') (interp ma) (fun a => interp (k a)) =
+        interp (mbind (M := M) ma k).
+    Proof.
+      induction ma; simpl; intros.
+      all: repeat rewrite ?mret_mbind, ?mbind_mret, ?mbind_mbind; s.
+    Qed.
+  End Free.
+End Free.
+
+Module Writer.
+Section Writer.
+  Context (T: Type).
+  Set Primitive Projections.
+  Record M A := { val: A; trace: list T }.
+  Unset Primitive Projections.
+
+  Local Definition ret {A} (a: A) : M A :=
+    {| val := a; trace := [] |}.
+  Local Definition bind {A B} (ma: M A) (k: A -> M B) : M B :=
+    let b := k ma.(val) in
+    {| val := b.(val); trace := b.(trace) ++ ma.(trace) |}.
+
+  Ltac s :=
+    unfold bind, ret; simpl;
+    rewrite ?List.app_nil_r, ?List.app_assoc;
+    firstorder congruence.
+
+  Global Program Instance MonadM : Monad M :=
+    {| mret := @ret;
+       mbind := @bind |}.
+  Obligation 2. Proof. s. Qed.
+  Obligation 3. Proof. s. Qed.
+End Writer.
+End Writer.
+
+Module Observable.
+  Import Writer.
+
+  Section Observable.
+  Context (T: Type).
+
+  Definition M A := Writer.M T A -> Prop.
+
+  (* FIXME: Combine nondeterminism with writer instead of defining from scratch *)
+  Definition ret {A} (a: A) : M A := fun r => r = {| val := a; trace := [] |}.
+  Definition bind {A B} (ma: M A) (k: A -> M B) : M B :=
+    fun obs =>
+      exists obsA obsB, ma obsA /\ k obsA.(val) obsB /\
+                   obs = {| val := obsB.(val);
+                            trace := obsA.(trace) ++ obsB.(trace) |}.
+
+  Ltac s :=
+    apply Ensembles.Extensionality_Ensembles;
+    unfold Ensembles.Same_set, Ensembles.Included, Ensembles.In;
+    repeat match goal with
+           | _ => reflexivity || eassumption
+           | _ => progress (intros; subst; simpl in * )
+           | [ H: exists _, _ |- _ ] => destruct H
+           | [ H: _ /\ _ |- _ ] => destruct H
+           | [  |- exists _, _ ] => eexists
+           | [  |- _ /\ _ ] => split
+           | _ => rewrite ?List.app_nil_r, ?List.app_assoc
+           end.
+
+  Global Program Instance MonadM : Monad M :=
+    {| mret {A} (a: A) := fun r => r = {| val := a; trace := [] |};
+       mbind {A B} (ma: M A) (k: A -> M B) :=
+         fun obs => exists obsA obsB, ma obsA /\ k obsA.(val) obsB /\
+                              obs = {| val := obsB.(val);
+                                       trace := obsB.(trace) ++ obsA.(trace) |} |}.
+  Obligation 1. Proof. s. Qed.
+  Obligation 2. Proof. s. Qed.
+  Obligation 3. Proof. s. Qed.
+  End Observable.
+End Observable.
+
+Module IO.
+  Import Writer.
+
+  Section IO.
+  Context (T: Type).
 
   Inductive Action : Type -> Type :=
   | Read : Action T
   | Write (w: T) : Action unit.
 
-  Definition IO := Free Action.
-  Definition ret {A} := @ret Action A.
-  Definition bind {A B} := @bind Action A B.
-  Definition bindn {A B} := @bindn Action A B.
-  Definition bind_ret {A} := @bind_ret A.
-  Definition ret_bind {A B} := @ret_bind A B.
-  Definition bind_bind {A B C} := @bind_bind A B C.
+  Definition M := (@Free.M Action).
+  (* Instance Monad : Monad (@Free.M Action) := @Free.Monad Action. *)
 
-  Inductive Event := R (t: T) | W (t: T).
-  Record Outcome {A} := { val: A; trace: list Event }.
-  Arguments Outcome : clear implicits.
+  Inductive Event T := R (t: T) | W (t: T).
 
-  Definition Observable A := Outcome A -> Prop.
-  Definition retObs {A} (a: A) : Observable A := fun r => r = {| val := a; trace := [] |}.
-  Definition bindObs {A B} (a: Observable A) (k: A -> Observable B) : Observable B :=
-    fun obs => exists obsA obsB, a obsA /\ k obsA.(val) obsB /\
-                         obs = {| val := obsB.(val);
-                                  trace := obsA.(trace) ++ obsB.(trace) |}.
-
-  Definition interpAction {A} (rw: Action A) : Observable A :=
+  Definition interpAction {A} (rw: Action A) : Observable.M (Event T) A :=
     match rw with
     | Read => fun out => out.(trace) = [R out.(val)]
     | Write w => fun out => out.(trace) = [W w]
     end.
 
-  Definition interpIO {A} (spec: IO A) : Observable A :=
-    interp Observable (@retObs) (@bindObs) (@interpAction) spec.
+  Definition interp {A} (spec: M A) : Observable.M (Event T) A :=
+    Free.interp (MM' := Observable.MonadM (Event T)) (@interpAction) spec.
 
-  Inductive ValidIO {A} : IO A -> Outcome A -> Prop :=
-    | ValidPure a : ValidIO (Pure a) {| val := a; trace := [] |}
+  Lemma interp_bind {A B}:
+    forall (ma: M A) (k: A -> M B),
+      mbind (interp ma) (fun a => interp (k a)) =
+      interp (mbind ma k).
+  Proof. intros; apply Free.interp_bind. Qed.
+
+  Inductive Valid {A} : IO.M A -> Writer.M (Event T) A -> Prop :=
+    | ValidPure a : Valid (Free.Pure a) {| val := a; trace := [] |}
     | ValidRead r k a t :
-        ValidIO (k r) {| val := a; trace := t |} ->
-        ValidIO (Impure Read k) {| val := a; trace := R r :: t |}
+        Valid (k r) {| val := a; trace := t |} ->
+        Valid (Free.Impure Read k) {| val := a; trace := t ++ [R r] |}
     | ValidWrite w k a t :
-        ValidIO (k tt) {| val := a; trace := t |} ->
-        ValidIO (Impure (Write w) k) {| val := a; trace := W w :: t |}.
+        Valid (k tt) {| val := a; trace := t |} ->
+        Valid (Free.Impure (Write w) k) {| val := a; trace := t ++ [W w] |}.
 
-  Hint Constructors ValidIO : io.
-  Lemma interpIO_ValidIO {A} (spec: IO A):
+  Hint Constructors Valid : io.
+  Lemma interp_Valid {A} (spec: IO.M A):
     forall obs,
-      ValidIO spec obs <-> interpIO spec obs.
+      Valid spec obs <-> interp spec obs.
   Proof.
-    induction spec; simpl; unfold retObs; intros.
+    induction spec; simpl; unfold Observable.ret; intros.
     - split; inversion 1; subst; eauto with io.
     - split.
       + inversion 1;
@@ -113,41 +181,35 @@ Module IOMonad.
                  | _ => progress subst
                  | [ H: existT _ _ _ = _ |- _ ] => apply Eqdep.EqdepTheory.inj_pair2 in H
                  end;
-          unfold bindObs.
+          unfold Observable.bind.
         1: exists {| val := r; trace := [R r] |}, {| val := a; trace := t |}.
         2: exists {| val := tt; trace := [W w] |}, {| val := a; trace := t |}.
         all: firstorder.
-      + destruct f; unfold bindObs;
+      + destruct f; unfold Observable.bind;
           repeat match goal with
                  | [ H: unit |- _ ] => destruct H
-                 | [ H: exists _: Outcome _, _ |- _ ] => destruct H as [(?&?) ?]
+                 | [ H: exists _: Writer.M _ _, _ |- _ ] => destruct H as [(?&?) ?]
                  | [ H: _ /\ _ |- _ ] => destruct H
-                 | [ H: Build_Outcome _ _ _ = _ |- _ ] => inversion H; subst; clear H
                  | _ => intros; subst; simpl in *
                  end.
-          all: firstorder eauto with io.
+        all: firstorder eauto with io.
   Qed.
-  End IOMonad.
+  End IO.
+End IO.
 
-  Arguments IO: clear implicits.
-  Arguments Action: clear implicits.
-  Arguments Event : clear implicits.
-  Arguments Outcome: clear implicits.
-End IOMonad.
-
-Import IOMonad.
+Arguments IO.Read {_} : assert.
 
 Notation "'let/!' x 'as' nm := val 'in' body" :=
-  (bindn [nm] (Call val) (fun x => body))
+  (mbindn [nm] (Free.Call val) (fun x => body))
     (at level 200, x ident, body at level 200,
      format "'[hv' 'let/!'  x  'as'  nm  :=  val  'in' '//' body ']'").
 
 Notation "'let/!' x := val 'in' body" :=
-  (bindn [IdentParsing.TC.ident_to_string x] (Call val) (fun x => body))
+  (mbindn [IdentParsing.TC.ident_to_string x] (Free.Call val) (fun x => body))
     (at level 200, x ident, body at level 200,
      only parsing).
 
-Require Import Coq.Init.Byte.
+Import Writer.
 
 Section with_parameters.
   Context {width: Z} {BW: Bitwidth width} {word: word.word width} {memT: map.map word Byte.byte}.
@@ -160,22 +222,15 @@ Section with_parameters.
   Context {ext_spec_ok : Semantics.ext_spec.ok ext_spec}.
 
   Context {T: Type}.
-  Notation IO := (IO T).
-  Notation Event := (Event T).
-  Notation Outcome := (Outcome T).
+  Notation IO := (IO.M T).
+  Notation Event := (IO.Event T).
+  Notation Writer := (Writer.M Event).
 
-  Definition iobind {A} (io: IO A) (pred: Outcome A -> Prop) :=
-    (* FIXME: how do I capture the fact that all permissible traces should be achievable? *)
-    exists out, ValidIO io out /\ pred out.
-
-  (* Lemma tbind_bindn {A B} (tr0: list Event) (pred: Outcome A -> predicate) *)
-  (*       vars (a: IO A) (k: A -> IO B) : *)
-  (*   tbind tr0 pred (bindn vars a k) = *)
-  (*   tbind (evf.(trace) ++ tr0) pred (k (evf.(val))). *)
-  (* Proof. *)
-  (*   unfold bindn, tbind, bind; simpl. *)
-  (*   rewrite app_assoc; reflexivity. *)
-  (* Qed. *)
+  Definition iobind {A} (io: IO A) (pred: Writer A -> Prop) :=
+    (* NOTE: We do not need to capture the fact that all traces are achievable:
+       Bedrock2 takes care of that for us (the source program has no control on the
+       values returned by "read" *)
+    exists out, IO.Valid io out /\ pred out.
 
   Definition trace_entry :=
     Eval cbv beta in ((fun {A} (_: list A) => A) _ ([]: Semantics.trace)).
@@ -188,6 +243,44 @@ Section with_parameters.
   Definition iospec_k {A} tr0 (pred: A -> predicate) (k: IO A) :=
     fun tr mem locals =>
       iospec tr0 k (fun a tr' => tr = tr' /\ pred a tr mem locals).
+
+  Arguments mret : simpl never.
+  Arguments mbind : simpl never.
+
+  Lemma iospec_k_bindn {A B} tr0 tr mem locals :
+    forall vars (fa : IO A) (k : A -> IO B) outa (pred : B -> predicate),
+      IO.Valid fa outa ->
+      iospec_k (List.map trace_entry_of_event outa.(trace) ++ tr0) pred (k outa.(val)) tr mem locals ->
+      iospec_k tr0 pred (mbindn vars fa k) tr mem locals.
+  Proof.
+    unfold iospec_k, iospec, iobind, mbindn; simpl.
+    intros vars * Hv (out & ? & -> & ?).
+    eexists {| val := out.(val); trace := out.(trace) ++ outa.(trace) |}.
+    repeat split; cbn.
+    - apply IO.interp_Valid in H, Hv.
+      apply IO.interp_Valid.
+      rewrite <- IO.interp_bind.
+      red; red; eauto.
+    - rewrite map_app, <- app_assoc; reflexivity.
+    - eassumption.
+  Qed.
+
+  Lemma WeakestPrecondition_iospec_k_bindn {A B} tr0 funcs prog tr mem locals :
+    forall vars (fa : IO A) (k : A -> IO B) outa (pred : B -> predicate),
+    IO.Valid fa outa ->
+    (IO.Valid fa outa ->
+     WeakestPrecondition.program
+       funcs prog tr mem locals
+       (iospec_k (List.map trace_entry_of_event outa.(trace) ++ tr0)
+                 pred (k outa.(val)))) ->
+    WeakestPrecondition.program
+      funcs prog tr mem locals
+      (iospec_k tr0 pred (mbindn vars fa k)).
+  Proof.
+    intros; eapply WeakestPrecondition_weaken.
+    - intros; eapply iospec_k_bindn; eauto.
+    - eauto.
+  Qed.
 
   (* FIXME: is there a way to avoid repeating `tr`? (The problem is that iospec_k needs to connect the traces produced by k and by the bedrock2 program.)
      Can running a program ever shrink the trace? *)
@@ -221,13 +314,12 @@ Section with_parameters.
     repeat match goal with
            | [ H: exists _, _ |- _ ] => destruct H
            | [ H: _ /\ _ |- _ ] => destruct H
-           | _ => subst
+           | _ => subst; eauto 6
            end.
-    eauto 6.
   Qed.
 End with_parameters.
 
 Global Hint Unfold iospec_k iospec iobind: compiler_cleanup.
-Global Hint Extern 1 (ret _ _) => reflexivity : compiler_cleanup.
+Global Hint Extern 1 (IO.Valid (mret _) _) => eapply IO.ValidPure : compiler_cleanup.
 Global Hint Resolve compile_setup_iospec : compiler_setup.
-Global Hint Extern 2 (IsRupicolaBinding (bindn _ _ _)) => exact true : typeclass_instances.
+Global Hint Extern 2 (IsRupicolaBinding (mbindn _ _ _)) => exact true : typeclass_instances.
